### Disproving experimental evidence

The velocity addition formula derivable from the Lorentz transformation, used as corroboration for the theory in subsequent experiments (e.g. Fizeau), derives a contradictory term for

$\frac{\partial x}{\partial t}$

to the constancy of light postulate Einstein uses to derive the Lorentz transformation.

$x = ct \rightarrow \frac{x}{t} = c$.

Then $\frac{\partial x}{\partial t} = c$ assuming uniform motion.

However, this contradicts the velocity addition formula:

$\frac{\partial x}{\partial t} = \frac{\frac{\partial x'}{\partial t'} + v}{1 + \frac{v}{c^2}\frac{\partial x'}{\partial t'}}$

for pretty much all experimentally tested velocities $W = \frac{\partial x}{\partial t} \neq c$.

### Deriving the velocity addition formula

Assume the Lorentz transformation. We have:

$\partial x = \frac{\partial x' + v \partial t'}{\sqrt{1 - \frac{v^2}{c^2}}}$

$\partial t = \frac{\partial t' + \frac{v \partial x'}{c^2}}{\sqrt{1 - \frac{v^2}{c^2}}}$

$\frac{\partial x}{\partial t} = \frac{\frac{\partial x' + v \partial t'}{\sqrt{1 - \frac{v^2}{c^2}}}}{\frac{\partial t' + \frac{v \partial x'}{c^2}}{\sqrt{1 - \frac{v^2}{c^2}}}} = \frac{\partial x' + v \partial t'}{\partial t' + \frac{v \partial x'}{c^2}} = \frac{\frac{1}{\partial t'}(\partial x' + v \partial t')}{\frac{1}{\partial t'}(\partial t' + \frac{v \partial x'}{c^2})} = \frac{\frac{\partial x'}{\partial t'} + v}{1 + \frac{v}{c^2}\frac{\partial x'}{\partial t'}}$
